demote wrongly classified message invariants into application invariants

networkInvariantPrototypes/paxos/applicationProof.dfy
@@ -20,6 +20,38 @@ predicate Chosen(c: Constants, v: Variables, vb: ValBal) {
   exists quorum: set<Message> :: IsAcceptQuorum(c, v, quorum, vb)
 }
 
+// Tony: I once thought this was a message invariant, but it isn't --- it depends on 
+// application level knowledge that l.receivedAccepts is monotonically increasing.
+// For every Learn(lnr, val) message in the network, the learner must have a quorum of
+// accepts for that val, at some common ballot
+predicate LearnMsgsValid(c: Constants, v: Variables)
+  requires v.WF(c)
+  requires ValidMessageSrc(c, v)
+{
+  forall lnr:LearnerId, bal, val | 
+    Learn(lnr, bal, val) in v.network.sentMsgs
+  :: 
+    && var vb := VB(val, bal);
+    && vb in v.learners[lnr].receivedAccepts
+    && |v.learners[lnr].receivedAccepts[vb]| >= c.f+1
+}
+
+// Tony: I once thought this was a message invariant, but it isn't --- it depends on 
+// application level knowledge that a.promised is monotonically increasing.
+// Every Promise message in the network has a ballot upper-bounded by the promised ballot
+// of the source acceptor
+predicate AcceptorPromisedMonotonic(c: Constants, v: Variables) 
+  requires v.WF(c)
+{
+  forall idx, prom | 
+    && c.ValidAcceptorIdx(idx) 
+    && IsPromiseMessage(v, prom)
+    && prom.acc == c.acceptorConstants[idx].id
+  ::
+    && v.acceptors[idx].promised.Some?
+    && prom.bal <= v.acceptors[idx].promised.value
+}
+
 predicate OneValuePerProposeBallot(c: Constants, v: Variables)
 {
   forall p1, p2 | 
@@ -170,6 +202,8 @@ predicate ApplicationInv(c: Constants, v: Variables)
   requires v.WF(c)
   requires MessageInv(c, v)
 {
+  && LearnMsgsValid(c, v)
+  && AcceptorPromisedMonotonic(c, v)
   && ProposeImpliesLeaderState(c, v)
   && PromiseVbImpliesAccepted(c, v)
   && AcceptMessageImpliesProposed(c, v)
@@ -593,6 +627,7 @@ lemma ChosenAndConflictingProposeImpliesFalse(c: Constants, v: Variables, chosen
 lemma LearnedImpliesChosen(c: Constants, v: Variables, learnMsg: Message)
   requires v.WF(c)
   requires MessageInv(c, v)
+  requires LearnMsgsValid(c, v)
   requires IsLearnMessage(v, learnMsg)
   ensures Chosen(c, v, VB(learnMsg.val, learnMsg.bal))
 {
